bedrock2-to-cava end-to-end theorem for IncrementWait (#814)
* sketch riscv machine model that concurrently runs a cava-defined device

* sketch deterministic executable RISC-V machine with Cava device

* we can now vm_compute the bedrock2-compiled IncrementWait
example on the deterministic riscv-coq machine with a
Cava increment circuit attached

* beware, `Hint Extern` without a pattern can lead to stack overflow
when running eg `Check (_ : Utility.Words)`

* put StateMachineMMIOSpec into separate file so that
MMIOToCava proof does not need to depend on MMIO compiler proof

* sketch statement connecting the compiler's riscv machine to
the riscv machine with a Cava device, and statement connecting
a bedrock2 program to the riscv machine with a Cava device

* update bedrock2 compiler to not using MemoryLayout any more

* prove bedrock2_and_cava_system_correct (but the interesting
part, stateMachine_to_cava_1, is still admitted)

* wip porting IncrementWait to new constants style
and generic StateMachineMMIO rather than IncrementWaitMMIO

* manually revert IncrementWait to using separate register for status

* document `device` typeclass

* cava incr device with separate VALUE/STATUS registers

* update IncrementWait proofs to generic StateMachineSemantics

* adding the right cut brings Qed time from seemingly infinite down to ~1sec

* replace `program` seplog assertion by `ptsto_bytes` of `instrencode`
in `bedrock2_and_cava_system_correct`, because `program` contains
"hidden" assumptions about the validity of the instructions emitted
by the compiler, which we want to appear as a separate hypothesis,
because the hypothesis "the memory contains the program" will not be
discharged inside Coq, so it shouldn't contain any hidden surprises

* include program logic soundness in bedrock2_and_cava_system_correct

* prove end-to-end theorem for IncrementWait (but important parts
like bridging between the compiler's RISC-V machine and the RISC-V
machine with the Cava device are still admitted)

* make sure machine_ok uses mmioAddr expressed in terms of lower
layer (ExtraRiscvMachine) rather than intermediate layer (which
is supposed to cancel out us much as possible)

* instead of requiring that the Cava device remembers the latest request,
pass the current request on the device's input wires

* define execution of risc-v machine with cava device as
interp of free monad (instead of directly using a Riscv monad
instance), so that we can prove the correspondence between
the compiler's risc-v machine and the cava risc-v machine for
each Riscv primitive separately, without having to go through
Run.run1 of all risc-v instructions.
However, this requires mid-conditions implying existence of
a state machine execution, and it's not clear how to make that
condition inductive.
Will probably have to require read_step/write_step in
mmioLoad/mmioStore of MinimalMMIO, instead of relying on post
asserting existence of an execution.

* add MMIOWriteOK and assert it in nonmem_store,
so that we get a `write_step` when inverting a MinimalMMIO risc-v
machine execution without having to rely on an `execution` in the
postcondition, which is not inductive

* use the MaterializeRiscvProgram.Materialize instance instead of
a metrics-specific instance (moving the metrics updating from the
RiscvProgram instance to the interp function), so that the compiler's
risc-v machine differs from the Cava risc-v machine only in its
interp function, which allows us to reason about their equivalence
at riscv_primitive granularity

* finish stateMachine_to_cava
(but still have to see if we can instantiate its assumptions,
device_implements_state_machine)

* moving the `device_implements_state_machine` instance for IncrementWait
to the file where the IncrementWait Cava circuit is defined,
splitting up a two-field parameter record along the way to avoid
having to define more parameter rewrapping instances, running into
a nasty usability issue (https://github.com/mit-plv/bedrock2/issues/193)
caused by Hint Mode + on map.map.

* first sketch of cava_counter_satisfies_state_machine,
still several problems in the device_state_related relation, but
already found and fixed two bugs in the Cava IncrementWait circuit:
- when the result value is read by the software, the device has to
  go back to IDLE
- the device must leave the IDLE state only if the request is a
  value write request, but stay in IDLE if the request is any other request

* don't rely on uniqueness of state machine execution any more
(but still require that it simulates a deterministic Cava device,
so there's only as much room for nondeterminism in the state machine
as allowed by the simulation relation)

* simplification/fixes related to initial states,
any_two_imply_the_third is not sufficient

* initial state conditions seem to work

* try to allow high-level underspecification nondeterminism in
state_machine_read/write_to_device_read/write, which seems
necessary to allow to not precisely specify in the high-level
state machine how many times we need to poll until the
device says that it went from BUSY to DONE.
Problem: Can't prove any more that the
(forall s, execution t s -> device_state_related s d)
condition of mkRelated is preserved, but still need it,
because we get one execution from the
(exists s, execution t s /\ device_state_related s d)
part in mkRelated for which we also get a device_state_related,
and another execution from mmioLoad, for which we don't get
a device_state_related, but need to construct one

* using execution_unique, the MMIO machine to Cava machine proof works again,
and still allows external high-level underspecification nondeterminism
(but not nondeterminism that's not immediately visible in the trace),
which is enough to prove that the Cava IncrementWait device implements the
IncrementWait state machine.
The IncrementWaitToCava end-to-end theorem is now almost admit-free:
Bbesides the propositional & functional extensionality axioms, there are
only three more admits, which all are uninteresting properties about words
(`naive_riscv_ok`, `incrN_word_to_bv` and `MMIOToCava.bv_to_word_word_to_bv`).

* cleanup

investigations/bedrock2/IncrementWait/IncrementWaitSemantics.v
@@ -3,6 +3,7 @@ Require Import Coq.micromega.Lia.
 Require Import Coq.Lists.List.
 Require Import Coq.Numbers.DecimalString.
 Require Import bedrock2.Syntax bedrock2.Semantics.
+Require Import bedrock2.ZnWords.
 Require coqutil.Datatypes.String coqutil.Map.SortedList.
 Require coqutil.Map.SortedListString coqutil.Map.SortedListWord.
 Require Import coqutil.Map.Interface.
@@ -12,6 +13,7 @@ Require Import coqutil.Z.HexNotation.
 Require Import coqutil.Decidable.
 Require Import Bedrock2Experiments.Word.
 Require Import Bedrock2Experiments.WordProperties.
+Require Import Bedrock2Experiments.StateMachineSemantics.
 Require Import Bedrock2Experiments.IncrementWait.Constants.
 
 Import String List.ListNotations.
@@ -24,24 +26,10 @@ Class circuit_behavior :=
   { ncycles_processing : nat
   }.
 
-Module parameters.
-  Class parameters :=
-    { word :> Interface.word.word 32;
-      mem :> Interface.map.map word Byte.byte;
-    }.
-
-  Class ok (p : parameters) :=
-    { word_ok :> word.ok word; (* for impl of mem below *)
-      mem_ok :> Interface.map.ok mem; (* for impl of mem below *)
-    }.
-End parameters.
-Notation parameters := parameters.parameters.
-
 Section WithParameters.
-  Context {p : parameters} {p_ok : parameters.ok p}.
-  Context {consts : constants word.rep} {consts_ok : constants_ok consts}
-          {circuit_spec : circuit_behavior}.
-  Import parameters.
+  Context {word: word.word 32} {word_ok: word.ok word}
+          {mem: map.map word Byte.byte} {mem_ok: Interface.map.ok mem}.
+  Context {circuit_spec : circuit_behavior}.
 
   Local Notation bedrock2_event := (mem * string * list word * (mem * list word))%type.
   Local Notation bedrock2_trace := (list bedrock2_event).
@@ -57,26 +45,25 @@ Section WithParameters.
 
   Definition reg_addr (r : Register) : word :=
     match r with
-    | VALUE => VALUE_ADDR
-    | STATUS => STATUS_ADDR
+    | VALUE => word.of_Z VALUE_ADDR
+    | STATUS => word.of_Z STATUS_ADDR
     end.
 
   Lemma reg_addrs_unique r1 r2 : reg_addr r1 = reg_addr r2 -> r1 = r2.
   Proof.
-    pose proof addrs_unique as Haddrs.
-    cbv [reg_addrs] in Haddrs. simplify_unique_words_in Haddrs.
-    destruct r1, r2; cbv [reg_addr]; congruence.
+    destruct r1, r2; cbv [reg_addr]; intros; try reflexivity;
+      exfalso; unfold VALUE_ADDR, STATUS_ADDR, INCR_BASE_ADDR in *; ZnWords.
   Qed.
 
   Definition status_flag (s : state) : word :=
     match s with
-    | IDLE => STATUS_IDLE
-    | BUSY _ _ => STATUS_BUSY
-    | DONE _ => STATUS_DONE
+    | IDLE => word.of_Z STATUS_IDLE
+    | BUSY _ _ => word.of_Z STATUS_BUSY
+    | DONE _ => word.of_Z STATUS_DONE
     end.
 
-  Definition status_value (flag : word) : word :=
-    word.slu (word.of_Z 1) flag.
+  Definition status_value (flag : Z) : word :=
+    word.slu (word.of_Z 1) (word.of_Z flag).
 
   (* circuit spec *)
   Definition proc : word -> word := word.add (word.of_Z 1).
@@ -112,104 +99,36 @@ Section WithParameters.
       end
     end.
 
-  Definition step
-             (action : string) (s : state) (args rets : list word) (s' : state)
-    : Prop :=
-    if String.eqb action WRITE
-    then match args with
-         | [addr;val] =>
-           (exists r, reg_addr r = addr /\ rets = [] /\ write_step s r val s')
-         | _ => False
-         end
-    else if String.eqb action READ
-         then match args with
-              | [addr] => (exists r val, reg_addr r = addr /\ rets = [val] /\ read_step s r val s')
-              | _ => False
-              end
-         else False.
+  Global Instance state_machine_parameters
+    : StateMachineSemantics.parameters 32 word mem :=
+    {| StateMachineSemantics.parameters.state := state ;
+       StateMachineSemantics.parameters.register := Register ;
+       StateMachineSemantics.parameters.is_initial_state := eq IDLE ;
+       StateMachineSemantics.parameters.read_step sz s a v s' :=
+         sz = 4%nat /\ read_step s a v s';
+       StateMachineSemantics.parameters.write_step sz s a v s' :=
+         sz = 4%nat /\ write_step s a v s' ;
+       StateMachineSemantics.parameters.reg_addr := reg_addr ;
+       StateMachineSemantics.parameters.isMMIOAddr a :=
+           INCR_BASE_ADDR <= word.unsigned a < INCR_END_ADDR;
+    |}.
 
-  (* Computes the Prop that must hold for this state to be accurate after the
-     trace *)
-  Fixpoint execution (t : bedrock2_trace) (s : state) : Prop :=
-    match t with
-    | [] => s = IDLE
-    | (_,action,args,(_,rets)) :: t =>
-      exists prev_state,
-      execution t prev_state
-      /\ step action prev_state args rets s
-    end.
-
-  Definition ext_spec (t : bedrock2_trace)
-             (mGive : mem)
-             (action : string)
-             (args: list word)
-             (post: mem -> list word -> Prop) :=
-    if String.eqb action WRITE
-    then
-      (exists r addr val,
-          args = [addr;val]
-          /\ mGive = map.empty
-          /\ reg_addr r = addr
-          (* there must exist *at least one* possible state given this trace,
-             and one possible transition given these arguments *)
-          /\ (exists s s', execution t s /\ write_step s r val s')
-          (* postcondition must hold for *all* possible states/transitions *)
-          /\ (forall s s',
-                execution t s ->
-                write_step s r val s' ->
-                post Interface.map.empty []))
-       else if String.eqb action READ
-            then
-              (exists r addr,
-                  args = [addr]
-                  /\ mGive = map.empty
-                  /\ reg_addr r = addr
-                  (* there must exist *at least one* possible state given this
-                     trace, and one possible transition given these arguments *)
-                  /\ (exists s s' val, execution t s /\ read_step s r val s')
-                  (* postcondition must hold for *all* possible states/transitions *)
-                  /\ (forall s s' val,
-                        execution t s ->
-                        read_step s r val s' ->
-                        post Interface.map.empty [val]))
-               else False.
-
-  Global Instance semantics_parameters  : Semantics.parameters :=
-    {|
-    Semantics.width := 32;
-    Semantics.word := parameters.word;
-    Semantics.mem := parameters.mem;
-    Semantics.locals := SortedListString.map _;
-    Semantics.env := SortedListString.map _;
-    Semantics.ext_spec := ext_spec;
-  |}.
-
-  Global Instance ext_spec_ok : ext_spec.ok _.
+  Global Instance state_machine_parameters_ok
+    : StateMachineSemantics.parameters.ok state_machine_parameters.
   Proof.
-    split;
-    cbv [ext_spec Semantics.ext_spec semantics_parameters
-    Morphisms.Proper Morphisms.respectful Morphisms.pointwise_relation Basics.impl
-    ];
-    intros.
-    all :
-    repeat match goal with
-           | H : context[(?x =? ?y)%string] |- _ =>
-             destruct (x =? y)%string in *
-           | H: exists _, _ |- _ => destruct H
-           | H: _ /\ _ |- _ => destruct H
-           | H : _ :: _  = _ :: _ |- _ => inversion H; clear H; subst
-           | H: False |- _ => destruct H
-           | H : reg_addr _ = reg_addr _ |- _ => apply reg_addrs_unique in H
-           | _ => progress subst
-           end; eauto 20 using Properties.map.same_domain_refl.
-  Qed.
-
-  Global Instance ok : Semantics.parameters_ok semantics_parameters.
-  Proof.
-    split; cbv [env locals mem semantics_parameters]; try exact _.
-    { cbv; auto. }
-    { exact (SortedListString.ok _). }
-    { exact (SortedListString.ok _). }
+    constructor;
+      unfold parameters.isMMIOAddr; cbn;
+      intros;
+      try exact _;
+      repeat match goal with
+             | H: _ /\ _ |- _ => destruct H
+             | r: Register |- _ =>
+               destruct r; cbn [reg_addr] in *; unfold VALUE_ADDR, STATUS_ADDR, INCR_BASE_ADDR in *
+             end;
+      subst;
+      eauto.
+    all: try ZnWords.
+    all: exfalso; ZnWords.
   Qed.
 
   (* COPY-PASTE this *)
