investigations/bedrock2/IncrementWait/CavaIncrementDevice.v
@@ -1,0 +1,324 @@
+Require Import Cava.Cava.
+Import Circuit.Notations.
+Require Import Cava.CavaProperties.
+
+
+Section WithCava.
+  Context {signal} {semantics : Cava signal}.
+
+  (* TODO doesn't Cava already provide these? *)
+  Definition ite{T: SignalType}(cond: signal Bit)(thn els: signal T):
+    cava (signal T) :=
+    branches <- packV (Vector.of_list [els; thn]);;
+    ctrl <- packV (Vector.of_list [cond]);;
+    indexAt branches ctrl.
+
+  Definition and3: signal Bit * signal Bit * signal Bit -> cava (signal Bit) :=
+    fun '(x1, x2, x3) => x12 <- and2 (x1, x2);; and2 (x12, x3).
+
+  Definition or3: signal Bit * signal Bit * signal Bit -> cava (signal Bit) :=
+    fun '(x1, x2, x3) => x12 <- or2 (x1, x2);; or2 (x12, x3).
+
+  Definition incr_update:
+    (* input: *)
+    signal Bit *             (* is_read_req *)
+    signal Bit *             (* is_write_req *)
+    signal (Vec Bit 32) *    (* req_addr (only relevant if is_reaq_req or is_write_req) *)
+    signal (Vec Bit 32) *    (* req_value (only relevant if is_write_req *)
+    (* state: *)
+    signal Bit *             (* idle *)
+    signal Bit *             (* busy *)
+    signal Bit *             (* done *)
+    signal (Vec Bit 32)      (* value *)
+    -> cava (
+    (* output: *)
+    signal Bit *             (* is_resp *)
+    signal (Vec Bit 32) *    (* resp (only relevant if is_resp *)
+    (* state: *)
+    signal Bit *             (* idle *)
+    signal Bit *             (* busy *)
+    signal Bit *             (* done *)
+    signal (Vec Bit 32))     (* value *)
+  := fun '(is_read_req, is_write_req, req_addr, req_value, idle, busy, done, value) =>
+       initialized <- or3 (idle, busy, done);;
+       idle <- ite initialized idle (constant true);;
+       is_resp <- or2 (is_read_req, is_write_req);;
+       (* bit #2 of the address determines if STATUS or VALUE register *)
+       req_addr1 <- Vec.tl req_addr;;
+       req_addr2 <- Vec.tl req_addr1;;
+       is_status_req <- Vec.hd req_addr2;;
+       is_value_req <- inv is_status_req;;
+       is_value_write_req <- and2 (is_value_req, is_write_req);;
+       isnt_value_write_req <- inv is_value_write_req;;
+       is_value_read_req <- and2 (is_value_req, is_read_req);;
+       no_pending_inp <- inv is_resp;;
+       result_ready <- or2 (busy, done);;
+       done2idle <- and2 (done, is_value_read_req);;
+       not_done2idle <- inv done2idle;;
+       idle2idle <- and2 (idle, isnt_value_write_req);;
+       idle' <- or2 (idle2idle, done2idle);;
+       busy' <- is_value_write_req;;
+       done' <- and2 (result_ready, not_done2idle);;
+       value_plus_one <- incrN value;;
+       value_or_input <- ite is_value_write_req req_value value;;
+       value' <- ite busy value_plus_one value_or_input;;
+       zeros <- Vec.const (constant false) 29;;
+       v1 <- Vec.cons done zeros;;
+       v2 <- Vec.cons busy v1;;
+       v3 <- Vec.cons idle v2;;
+       resp <- ite is_status_req v3 value;;
+       ret (is_resp, resp, idle', busy', done', value').
+
+  Definition incr: Circuit (signal Bit * signal Bit * signal (Vec Bit 32) * signal (Vec Bit 32))
+                           (signal Bit * signal (Vec Bit 32)) :=
+    Loop (Loop (Loop (Loop (Comb incr_update)))).
+
+End WithCava.
+
+Definition incr_device_step:
+  (* input: current state, is_read_req, is_write_req, req_addr, req_value *)
+  circuit_state incr -> bool * bool * Bvector 32 * Bvector 32 ->
+  (* output: next state, is_resp, resp *)
+  circuit_state incr * (bool * Bvector 32)
+  := step incr.
+
+Require Import coqutil.Datatypes.List.
+
+(* like `simulate`, but also output the internal state, for more insightful debugging *)
+Fixpoint simulate_with_state_rec{i o}(c: Circuit i o)(initial: circuit_state c)(inps: list i)
+  : list (circuit_state c * o) :=
+  match inps with
+  | [] => []
+  | inp :: rest => let r := step c initial inp in r :: simulate_with_state_rec c (fst r) rest
+  end.
+Definition simulate_with_state{i o}(c: Circuit i o): list i -> list (circuit_state c * o) :=
+  simulate_with_state_rec c (reset_state c).
+
+Example sample_trace := Eval compute in simulate_with_state incr [
+  (false, false, N2Bv_sized 32 111, N2Bv_sized 32 111); (* no action *)
+  (false, true, N2Bv_sized 32 0, N2Bv_sized 32 15);     (* write VALUE:=15 *)
+  (true, false, N2Bv_sized 32 4, N2Bv_sized 32 111);    (* read STATUS *)
+  (true, false, N2Bv_sized 32 4, N2Bv_sized 32 111);    (* read STATUS *)
+  (true, false, N2Bv_sized 32 0, N2Bv_sized 32 111)     (* read VALUE *)
+].
+
+(* Print sample_trace. *)
+
+Require Import Coq.ZArith.ZArith. Open Scope Z_scope.
+Require Import riscv.Utility.Utility.
+Require Import coqutil.Map.Interface coqutil.Map.Properties.
+Require Import coqutil.Word.Interface coqutil.Word.Properties.
+Require Import coqutil.Tactics.Simp.
+Require Import bedrock2.ZnWords.
+Require Import Bedrock2Experiments.RiscvMachineWithCavaDevice.InternalMMIOMachine.
+Require Import Bedrock2Experiments.IncrementWait.Constants.
+Require Import Bedrock2Experiments.IncrementWait.IncrementWaitSemantics.
+Require Import Bedrock2Experiments.RiscvMachineWithCavaDevice.MMIOToCava.
+
+Section WithParameters.
+  Context {word: Interface.word 32} {word_ok: word.ok word}
+          {Mem: map.map word byte} {Registers: map.map Z word}.
+
+  Definition mk_counter_state(idle busy done: bool)(val: Bvector 32): circuit_state incr :=
+    (tt, (tt, (tt, (tt, (tt, val), done), busy), idle)).
+
+  Global Instance counter_device: device := {|
+    device.state := circuit_state incr;
+    device.is_ready_state s := exists val idle, s = mk_counter_state idle false false val;
+    device.run1 := incr_device_step;
+    device.addr_range_start := INCR_BASE_ADDR;
+    device.addr_range_pastend := INCR_END_ADDR;
+    device.maxRespDelay := 1;
+  |}.
+
+  (* conservative upper bound matching the instance given in IncrementWaitToRiscv *)
+  Global Instance circuit_spec : circuit_behavior :=
+  {| ncycles_processing := 15%nat |}.
+
+  Ltac destruct_state s :=
+    destruct s as ([] & (([] & (([] & (([] & ([] & ?val)) & ?done)) & ?busy)) & ?idle)).
+
+  Inductive counter_related: IncrementWaitSemantics.state -> circuit_state incr -> Prop :=
+  | IDLE_related: forall val idle,
+      (* after reset, all three bools are false, and idle will be set to true *)
+      counter_related IDLE (mk_counter_state idle false false val)
+  | BUSY_related: forall val ncycles,
+      (0 < ncycles)%nat ->
+      counter_related (BUSY val ncycles) (mk_counter_state false true false (word_to_bv val))
+  (* the hardware is already done, but the software hasn't polled it yet to find out,
+     so we have to relate a software-BUSY to a hardware-done: *)
+  | BUSY_done_related: forall val ncycles,
+      counter_related (BUSY val ncycles)
+                      (mk_counter_state false false true (word_to_bv (word.add (word.of_Z 1) val)))
+  | DONE_related: forall val,
+      counter_related (DONE val) (mk_counter_state false false true (word_to_bv val)).
+
+  Axiom TODO: False.
+
+  Axiom word_to_bv_inj: forall x y, word_to_bv x = word_to_bv y -> x = y.
+
+  Axiom incrN_word_to_bv: forall v, incrN (word_to_bv v) = word_to_bv (word.add (word.of_Z 1) v).
+
+  Set Printing Depth 100000.
+
+  Global Instance cava_counter_satisfies_state_machine:
+    device_implements_state_machine counter_device state_machine_parameters.
+  Proof.
+    eapply Build_device_implements_state_machine with (device_state_related := counter_related);
+      intros.
+    - (* mmioAddrs_match: *)
+      reflexivity.
+    - (* initial_state_is_ready_state: *)
+      simpl in *. subst. inversion H0. eauto.
+    - (* initial_states_are_related: *)
+      simpl in *. destruct H0 as (val & idle & H0). subst. eapply IDLE_related.
+    - (* initial_state_exists: *)
+      simpl in *. destruct H as (val & idle & H). subst. eauto using IDLE_related.
+    - (* nonMMIO_device_step_preserves_state_machine_state: *)
+      simpl in sL1, sL2. destruct_state sL1. destruct_state sL2.
+      cbn [device.run1 counter_device incr_device_step step incr incr_update Loop snd
+           ret bind monad CombinationalSemantics Identity.Monad_ident constant] in H0.
+      eapply pair_equal_spec in H0. destruct H0 as [E1 E2].
+      subst.
+      eapply pair_equal_spec in E1. destruct E1 as [_ E1].
+      eapply pair_equal_spec in E1. destruct E1 as [E1 E2]. simpl in E2. subst.
+      eapply pair_equal_spec in E1. destruct E1 as [_ E1].
+      eapply pair_equal_spec in E1. destruct E1 as [E1 E2]. simpl in E2. subst.
+      eapply pair_equal_spec in E1. destruct E1 as [_ E1].
+      eapply pair_equal_spec in E1. destruct E1 as [E1 E2]. simpl in E2. subst.
+      eapply pair_equal_spec in E1. destruct E1 as [_ E1].
+      eapply pair_equal_spec in E1. destruct E1 as [_ E1]. simpl in E1. subst.
+      inversion H; subst.
+      + (* IDLE_related: *)
+        cbn. rewrite andb_false_r. destruct idle; cbn; simpl; eapply IDLE_related.
+      + (* BUSY_related: *)
+        rewrite andb_false_r. cbn -[incrN]. change (Pos.to_nat 1) with 1%nat.
+        cbn -[incrN]. rewrite incrN_word_to_bv.
+        eapply BUSY_done_related.
+      + (* BUSY_done_related: *)
+        cbn. rewrite andb_false_r. cbn. assumption.
+      + (* DONE_related: *)
+        cbn. rewrite andb_false_r. cbn. assumption.
+    - (* state_machine_read_to_device_read: *)
+      (* simpler because device.maxRespDelay=1 *)
+      unfold device.maxRespDelay, device.runUntilResp, device.state, device.run1, counter_device.
+      unfold StateMachineSemantics.parameters.read_step, state_machine_parameters in *.
+      simp.
+      unfold read_step in *.
+      destruct r.
+      + (* r=VALUE *)
+        simp.
+        cbn. rewrite andb_false_r. simpl.
+        unfold word_to_bv. rewrite word.unsigned_of_Z_nowrap by (cbv; intuition discriminate).
+        simpl. do 3 eexists. ssplit; try reflexivity. eapply IDLE_related.
+      + (* r=STATUS *)
+        destruct sH.
+        * (* sH=IDLE *)
+          destruct Hp1. subst. inversion H0. subst.
+          cbn. rewrite andb_false_r. simpl. unfold status_value, STATUS_IDLE.
+          unfold word_to_bv.
+          rewrite word.unsigned_of_Z_nowrap by (cbv; intuition discriminate).
+          do 3 eexists. ssplit; try reflexivity. 2: eapply IDLE_related.
+          rewrite word.unsigned_slu. 2: rewrite word.unsigned_of_Z. 2: reflexivity.
+          rewrite !word.unsigned_of_Z. unfold word.wrap. cbn.
+          destruct idle; reflexivity.
+        * (* sH=BUSY *)
+          simp.
+          destruct Hp1 as [H | H].
+          -- (* transition to DONE *)
+             destruct H; subst.
+             simpl (StateMachineSemantics.parameters.reg_addr _).
+             unfold STATUS_ADDR, INCR_BASE_ADDR, word_to_bv, status_value, STATUS_DONE.
+             rewrite !word.unsigned_of_Z. unfold word.wrap. simpl.
+             inversion H0; subst.
+             ++ (* BUSY_related *)
+                (* the transition that was used to show that sH is not stuck was a transition
+                   from BUSY to DONE returning a done flag, but since the device is still
+                   in BUSY state, it will still return the busy flag in this transition,
+                   so the transition we use to simulate what happened in the device is a
+                   BUSY-to-DONE transition returning a busy flag instead of a done flag *)
+                destruct max_cycles_until_done. 1: inversion H3. clear H3.
+                exists (word.of_Z 2). (* <- bit #1 (busy) is set, all others are 0 *)
+                do 2 eexists.
+                rewrite !word.unsigned_of_Z. unfold word.wrap. cbn -[incrN].
+                ssplit; try reflexivity.
+                ** simpl. rewrite incrN_word_to_bv. eapply BUSY_done_related.
+                ** right. eexists; ssplit; try reflexivity. eapply word.unsigned_inj.
+                   rewrite word.unsigned_slu. 2: rewrite word.unsigned_of_Z. 2: reflexivity.
+                   rewrite !word.unsigned_of_Z. reflexivity.
+             ++ (* BUSY_done_related *)
+                exists (word.of_Z 4). (* <- bit #2 (done) is set, all others are 0 *)
+                do 2 eexists.
+                rewrite !word.unsigned_of_Z. unfold word.wrap. cbn -[incrN].
+                ssplit; try reflexivity.
+                ** simpl. eapply DONE_related.
+                ** left. split. 2: reflexivity. eapply word.unsigned_inj.
+                   rewrite word.unsigned_slu. 2: rewrite word.unsigned_of_Z. 2: reflexivity.
+                   rewrite !word.unsigned_of_Z. reflexivity.
+          -- (* stay BUSY *)
+             destruct H as (n & ? & ? & ?); subst.
+             simpl (StateMachineSemantics.parameters.reg_addr _).
+             unfold STATUS_ADDR, INCR_BASE_ADDR, word_to_bv, status_value, STATUS_BUSY.
+             rewrite !word.unsigned_of_Z. unfold word.wrap. simpl.
+             inversion H0; subst.
+             ++ (* BUSY_related *)
+                exists (word.of_Z 2). (* <- bit #1 (busy) is set, all others are 0 *)
+                do 2 eexists.
+                rewrite !word.unsigned_of_Z. unfold word.wrap. cbn -[incrN].
+                ssplit; try reflexivity.
+                ** simpl. rewrite incrN_word_to_bv. eapply BUSY_done_related.
+                ** right. eexists; ssplit; try reflexivity. eapply word.unsigned_inj.
+                   rewrite word.unsigned_slu. 2: rewrite word.unsigned_of_Z. 2: reflexivity.
+                   rewrite !word.unsigned_of_Z. reflexivity.
+             ++ (* BUSY_done_related *)
+                (* the transition that was used to show that sH is not stuck was a transition
+                   from BUSY to BUSY returning a busy flag, but since the device already is
+                   in done state, it will return a done flag in this transition,
+                   so the transition we use to simulate what happened in the device is a
+                   BUSY-to-DONE transition returning a done flag instead of a
+                   BUSY-to-BUSY transition returning a busy flag. *)
+                exists (word.of_Z 4). (* <- bit #2 (done) is set, all others are 0 *)
+                do 2 eexists.
+                rewrite !word.unsigned_of_Z. unfold word.wrap. cbn -[incrN].
+                ssplit; try reflexivity.
+                ** simpl. eapply DONE_related.
+                ** left. split. 2: reflexivity. eapply word.unsigned_inj.
+                   rewrite word.unsigned_slu. 2: rewrite word.unsigned_of_Z. 2: reflexivity.
+                   rewrite !word.unsigned_of_Z. reflexivity.
+        * (* sH=DONE *)
+          destruct Hp1. subst. inversion H0. subst.
+          simpl (StateMachineSemantics.parameters.reg_addr _).
+          unfold STATUS_ADDR, INCR_BASE_ADDR, word_to_bv, status_value, STATUS_DONE.
+          cbn.
+          rewrite !word.unsigned_of_Z. unfold word.wrap. cbn -[Vec.hd Vec.tl incrN].
+          exists (word.of_Z 4). (* <- bit #2 (done) is set, all others are 0 *)
+          do 2 eexists.
+          rewrite !word.unsigned_of_Z. unfold word.wrap. cbn.
+          ssplit; try reflexivity.
+          ** simpl. eapply DONE_related.
+          ** eapply word.unsigned_inj.
+             rewrite word.unsigned_slu. 2: rewrite word.unsigned_of_Z. 2: reflexivity.
+             rewrite !word.unsigned_of_Z. reflexivity.
+    - (* state_machine_write_to_device_write: *)
+      destruct H as (sH' & ? & ?). subst.
+      unfold write_step in H1.
+      destruct r. 2: contradiction.
+      destruct sH; try contradiction. subst.
+      inversion H0. subst.
+      cbn.
+      unfold word_to_bv.
+      rewrite word.unsigned_of_Z_nowrap by (cbv; intuition discriminate).
+      cbn.
+      eexists _, _, _. ssplit; try reflexivity. destruct idle; eapply BUSY_related; lia.
+    - (* read_step_unique: *)
+      cbn in *. unfold read_step in *. simp.
+      destruct v; destruct r; try contradiction; simp; try reflexivity.
+      destruct Hp1; destruct H0p1; simp; try reflexivity;
+        unfold status_value in *; exfalso; ZnWords.
+    - (* write_step_unique: *)
+      cbn in *. unfold write_step in *. simp. subst. reflexivity.
+    - (* initial_state_unique: *)
+      cbn in *. subst. reflexivity.
+  Qed.
+
+End WithParameters.
