investigations/bedrock2/IncrementWait/RunIncrementWaitSoftwareOnCava.v
@@ -1,0 +1,102 @@
+Require Import Coq.ZArith.ZArith.
+Require Import Coq.Lists.List. Import ListNotations.
+Require Import coqutil.Datatypes.List.
+Require Import coqutil.Word.Interface coqutil.Map.Interface.
+Require Import coqutil.Map.OfListWord.
+Require Import Bedrock2Experiments.RiscvMachineWithCavaDevice.InternalMMIOMachine.
+Require Import Bedrock2Experiments.IncrementWait.IncrementWaitToRiscV.
+Require Import Bedrock2Experiments.IncrementWait.CavaIncrementDevice.
+Require Import riscv.Spec.Decode.
+Require Import riscv.Utility.InstructionCoercions.
+Open Scope ilist_scope.
+Require Import compiler.MemoryLayout.
+
+Definition ml: MemoryLayout := {|
+  MemoryLayout.code_start    := word.of_Z 0;
+  MemoryLayout.code_pastend  := word.of_Z (4*2^10);
+  MemoryLayout.heap_start    := word.of_Z (4*2^10);
+  MemoryLayout.heap_pastend  := word.of_Z (8*2^10);
+  MemoryLayout.stack_start   := word.of_Z (8*2^10);
+  MemoryLayout.stack_pastend := word.of_Z (16*2^10);
+|}.
+
+Definition main_relative_pos :=
+  match map.get (snd (fst put_wait_get_compile_result)) (fst main) with
+  | Some p => p
+  | None => -1111
+  end.
+
+Definition p_call: Utility.word :=
+  word.add ml.(code_start) (word.of_Z (4 * Z.of_nat (List.length put_wait_get_asm))).
+
+Definition p_functions: Utility.word := ml.(code_start).
+
+Definition all_insts: list Instruction :=
+  put_wait_get_asm ++ [[ Jal RegisterNames.ra
+            (main_relative_pos + word.signed (word.sub p_functions p_call))]].
+
+Definition initial: ExtraRiscvMachine counter_device := {|
+  getMachine := {|
+    getRegs := map.put (map.of_list (List.map (fun n => (Z.of_nat n, word.of_Z 0)) (List.seq 0 32)))
+                       RegisterNames.sp ml.(stack_pastend);
+    getPc := p_call;
+    getNextPc := word.add p_call (word.of_Z 4);
+    getMem := (map.putmany (map.of_list_word_at ml.(code_start) (Pipeline.instrencode all_insts))
+              (map.putmany (map.of_list_word_at (word.sub ml.(stack_pastend) (word.of_Z 512))
+                                                (List.repeat Byte.x00 512))
+              (map.of_list_word_at ml.(heap_start)
+                        (HList.tuple.to_list (LittleEndian.split 4 42) ++
+                         HList.tuple.to_list (LittleEndian.split 4 12345678)))));
+    getXAddrs := List.map (fun n => word.add ml.(code_start) (word.of_Z (Z.of_nat n)))
+                          (List.seq 0 (4 * List.length all_insts));
+    getLog := [];
+  |};
+  getExtraState := Circuit.reset_state incr;
+|}.
+
+Definition sched: schedule := fun n => (n mod 2)%nat.
+
+Definition force_ow32(ow32: option Utility.w32): Z :=
+  match ow32 with
+  | Some v => LittleEndian.combine 4 v
+  | None => -1
+  end.
+
+Definition get_output(m: ExtraRiscvMachine counter_device): Z :=
+  force_ow32 (Memory.loadWord m.(getMachine).(getMem) (word.of_Z (width:=32) output_ptr)).
+
+Definition LogElem := (bool * Z * Z)%type. (* (ok-flag, pc, output) triples *)
+
+Definition outcomeToLogElem(outcome: option unit * ExtraRiscvMachine counter_device): LogElem :=
+  (match fst outcome with
+   | Some _ => true
+   | None => false
+   end,
+   word.unsigned (snd outcome).(getMachine).(getPc),
+   get_output (snd outcome)).
+
+Fixpoint trace(nsteps: nat)(start: ExtraRiscvMachine counter_device):
+  ExtraRiscvMachine counter_device * list (bool * Z * Z) :=
+  match nsteps with
+  | O => (start, [])
+  | S n => let (m, t) := trace n start in
+           let (o, m') := nth_step sched n m in
+           (m', t ++ [(match o with
+                       | Some tt => true
+                       | None => false
+                       end,
+                       word.unsigned m'.(getMachine).(getPc),
+                       get_output m')])
+  end.
+
+(* Useful for debugging: display (ok-flag, pc, output) after each cycle:
+Compute snd (trace 100 initial).
+*)
+
+Definition res(nsteps: nat): (bool * Z * Z) := outcomeToLogElem (run sched nsteps initial).
+
+(* We can vm_compute through the execution of the IncrementWait program,
+   riscv-coq's processor model, and Cava's reaction to the IncrementWait program: *)
+Goal exists nsteps, res nsteps = (true, word.unsigned p_call + 4, 43).
+  exists 82%nat. vm_compute. reflexivity.
+Qed.
